refactor: move environment def to Assumption.lean, move straight-line semantics to relevant modules

EffectSSA/ProofSketch/Assumptions.lean
@@ -7,6 +7,10 @@ public import EffectSSA.ProofSketch.Notation.Refinement
 namespace EffectSSA.ProofSketch
 public section
 
+/-!
+## SSA Assumptions
+-/
+
 class SSA (ι : Type) (σ : outParam Type) (ν : outParam Type) : Type where
   [decidableEq : DecidableEq ι]
   [stateRefine : Refinement σ]
@@ -19,6 +23,91 @@ attribute [implicit_reducible, instance]
 
 @[reducible] instance SSA.instDenote [ssa : SSA ι σ ν] : Denote ι (σ → List ν → σ × List ν) where
   denote := ssa.denoteInst
+
+/-!
+## Environment
+-/
+section Env
+variable [SSA ι σ ν]
+
+/--
+A local environment is a partial map from variables to values.
+-/
+structure LocalEnv (ι) {σ ν} [SSA ι σ ν] : Type where
+  get? : VarId → Option ν := fun _ => none
+
+instance : CoeFun (LocalEnv ι) (fun _ => VarId → Option ν) where
+  coe := LocalEnv.get?
+
+/--
+A stateful environment `ρ : SEnv` consists of a
+- local environment, a
+- global state, and
+- an error flag
+-/
+structure SEnv (ι) {σ ν} [ssa : SSA ι σ ν] : Type where
+  /-- A partial map from local variables (i.e, virtual registers) to values. -/
+  locals : LocalEnv ι := { }
+  /-- The global state, e.g, for memory and UB -/
+  state : σ := ssa.initialState
+  /-- Whether an interpretation occurred (indicating a mallformed program). -/
+  error : Bool := false
+
+/--
+`getD (some ρ)` returns `ρ`, `getD none` returns a default environment
+with the `error` flag set. -/
+abbrev SEnv.getD : Option (SEnv ι) → SEnv ι :=
+  (Option.getD · { error := true})
+
+/-! ### LocalEnv API -/
+namespace LocalEnv
+
+/--
+`ℓ.with? xs vs` returns the local environment `ℓ` with each variable `xs[i]`
+set to the corresponding value `vs[i]`,
+returining `none` if `xs` and `vs` are of different lengths.
+-/
+def with? (ℓ : LocalEnv ι) (xs : List VarId) (vs : List ν) : Option (LocalEnv ι) :=
+  if xs.length != vs.length then
+    none
+  else
+    some { get? x :=
+      match xs.idxOf? x with
+      | some idx => vs[idx]?
+      | none => ℓ x
+    }
+
+def «with» (ℓ : LocalEnv ι) (x : VarId) (v : ν) : LocalEnv ι where
+  get? y := if x = y then v else ℓ y
+
+section Lemmas
+variable (ℓ : LocalEnv ι)
+
+@[ext, grind ext]
+theorem ext {ℓ κ : LocalEnv ι} (h : ∀ x, ℓ x = κ x) : ℓ = κ := by
+  cases ℓ; cases κ; congr; funext x; apply h x
+
+@[simp, grind =]
+theorem with?_cons_cons : ℓ.with? (x :: xs) (v :: vs) = (·.with x v) <$> ℓ.with? xs vs := by
+  simp only [with?, List.length_cons, Nat.reduceBneDiff, bne_iff_ne, ne_eq, ite_not]
+  by_cases hl : xs.length = vs.length
+  case neg => grind
+  case pos =>
+    simp only [hl, ↓reduceIte, Option.map_eq_map, Option.map_some, Option.some.injEq]
+    congr 1; funext y
+    grind
+
+@[simp, grind =]
+theorem with?_nil_nil : ℓ.with? [] [] = some ℓ := by
+  simp [with?]
+
+@[simp, grind =] theorem get?_with :
+    (ℓ.with x v).get? y = if x = y then some v else ℓ y := by rfl
+
+
+end Lemmas
+end LocalEnv
+end Env
 
 /-!
 ## Axiomatized SSA Instance
